

Motivation: infinite sequence of independent trials with probability  $p$  (of success)

$N$  = # trials needed to see the first success.

$$P(N=k) = \underline{(1-p)^{k-1} p}$$

one way to think about this...

$$X_j = \begin{cases} 1 & \text{if trial } j \text{ is a success} \\ 0 & \text{if failure} \end{cases}$$

$$\begin{aligned} P(X_1=0, X_2=0, \dots, X_{k-1}=0, X_k=1) \\ &= P(X_1=0) P(X_2=0) \dots P(X_{k-1}=0) P(X_k=1) \\ &= (1-p) \dots (1-p) p. \end{aligned}$$

Def'n: let  $0 < p \leq 1$ . A random variable  $X$  has the geometric distribution with success parameter  $p$  if the possible values of  $X$  are  $\{1, 2, 3, \dots\}$  and  $P(X=k) = (1-p)^{k-1} p$ .

Remark: Sometimes define  $Y = X - 1$ .  $\boxed{X \sim \text{Geom}(p)}$   
possible values of  $Y$  are  $0, 1, 2, \dots$   
 $Y$  = # of failures before first success.

Ex: What is the probability that it takes more than 7 rolls of a fair die to roll a 6?

Sol'n:  $N = \#$  of rolls of a fair die until the first 6.

$$\begin{aligned} P(N > 7) &= \sum_{k=8}^{\infty} P(N=k) \\ &= \sum_{k=8}^{\infty} \left(\frac{5}{6}\right)^{k-1} \left(\frac{1}{6}\right) \\ &= \frac{1}{6} \sum_{k=8}^{\infty} \left(\frac{5}{6}\right)^{k-1} \\ &= \frac{1}{6} \frac{\left(\frac{5}{6}\right)^7}{1 - \frac{5}{6}} \\ &= \left(\frac{5}{6}\right)^7. \end{aligned}$$

Alternate: want first 7 rolls to be a failure.  $\left(\frac{5}{6}\right)^7$

Ex: Roll a pair of fair dice until you get either a sum of 5 or a sum of 7.  
 What is the probability that you get 5 first?

Sol'n: A: the event that 5 comes first.

$A_n = \{ \text{no 5 or 7 in first } n-1 \text{ rolls, and 5 on roll } n \}$ .

$$A = \bigcup_n A_n. \quad (1-(a+b))^{n-1} \cdot a$$

$$P(A) = \sum_n P(A_n).$$

$$P(A_n) = \left[ P(\text{no 5 or 7 on a roll}) \right]^{n-1} \cdot P(5 \text{ on roll } n)$$

$$\begin{aligned} P(\text{pair of dice gives 5}) &= \frac{4}{36} = a = \frac{1}{9} \\ P(\text{pair of dice gives 7}) &= \frac{6}{36} = b = \frac{1}{6} \\ \text{or } &= \left(1 - \frac{10}{36}\right)^{n-1} \left(\frac{4}{36}\right) \quad \leftarrow \text{where geom dist shows up.} \end{aligned}$$

$$P(A) = \frac{1}{9} \sum_n \left(1 - \frac{10}{36}\right)^{n-1} = \frac{1}{9} \sum_{n=1}^{\infty} \left(\frac{23}{36}\right)^{n-1}$$

$$= \frac{1}{9} \cdot \frac{1}{1 - \frac{13}{18}} = \frac{2}{5}$$

$$P(A) = \sum_{n=1}^{\infty} (1 - (a+b))^{n-1} a$$

$$= a \cdot \frac{1}{1 - (1 - (a+b))} = \frac{a}{a+b}$$

In this example,  $\frac{a}{a+b} = \frac{4/36}{\frac{4}{36} + \frac{6}{36}}$

$$= \frac{4}{4+6} = \frac{2}{5}$$

Expected Value of Geom. Distribution.

$X$  discrete rv

$$E(X) = \sum_k k P(X=k) \quad (q \stackrel{\text{def}}{=} 1-p)$$

$$X \sim \text{Geom}(p), \quad 0 < p < 1. \quad \checkmark$$

$$P(X=k) = (1-p)^{k-1} p = q^{k-1} p$$

$$E(X) = p \sum_{k=1}^{\infty} k q^{k-1}.$$

If  $|t| < 1$

$$\begin{aligned} \underbrace{\sum_{k=1}^{\infty} k t^{k-1}}_{1 + 2t + 3t^2 + \dots} &= \sum_{k=0}^{\infty} \frac{d}{dt} (t^k) \\ &= \frac{d}{dt} \left( \sum_{k=0}^{\infty} t^k \right) \quad \downarrow \text{Analysis fact} \\ &= \frac{d}{dt} \left( \frac{1}{1-t} \right) \\ &= \frac{1}{(1-t)^2} \end{aligned}$$

Then

$$E(X) = p \sum_{k=1}^{\infty} k q^{k-1} = \frac{p}{(1-q)^2} = \frac{p}{p^2} = \left( \frac{1}{p} \right).$$